tests/lean/Tutorial/Proofs.lean
@@ -1,8 +1,80 @@
 import Base
-open Primitives
-open Result
+open Primitives Result
+
+namespace Primitives
+
+end Primitives
 
 namespace Tutorial
+
+def times4 (x : U32) : Result U32 := do
+  let x1 ← x + x
+  x1 + x1
+
+def times16 (x : U32) : Result U32 := do
+  let x1 ← times4 x
+  times4 x1
+
+#check U32.add_spec
+
+-- Without progress
+theorem times4_spec (x : U32) (h : 4 * x.val ≤ U32.max) :
+  times4 x = ok (4 * x)#u32 := by
+  rw [times4]
+  have ⟨ x1, hEq1, hPost1 ⟩ := @U32.add_spec x x (by scalar_tac)
+  simp [hEq1]
+  have ⟨ x2, hEq2, hPost2 ⟩ := @U32.add_spec x1 x1 (by scalar_tac)
+  simp [hEq2]
+  scalar_tac
+
+-- With progress
+@[pspec]
+theorem times4_spec1 (x : U32) (h : 4 * x.val ≤ U32.max) :
+  times4 x = ok (4 * x)#u32 := by
+  rw [times4]
+  progress
+  progress
+  scalar_tac
+
+theorem times16_spec (x : U32) (h : 16 * x.val ≤ U32.max) :
+  times16 x = ok (16 * x)#u32 := by
+  rw [times16]
+  progress
+  progress
+  scalar_tac
+
+/- [demo::incr]:
+   Source: 'tests/src/demo.rs', lines 23:0-23:31 -/
+def incr (x : U32) : Result U32 :=
+  x + 1#u32
+
+/- [demo::use_incr]:
+   Source: 'tests/src/demo.rs', lines 27:0-27:17 -/
+def use_incr : Result Unit :=
+  do
+  let x ← incr 0#u32
+  let x1 ← incr x
+  let _ ← incr x1
+  Result.ok ()
+
+divergent def i32_id (n : I32) : Result I32 :=
+  if n = 0#i32 then ok 0#i32
+  else do
+    let n1 ← n - 1#i32
+    let n2 ← i32_id n1
+    n2 + 1#i32
+
+theorem i32_id_spec (n : I32) (h : 0 ≤ n.val) :
+  i32_id n = ok n := by
+  rw [i32_id]
+  split
+  . simp [*]
+  . progress as ⟨ n1 ⟩
+    progress
+    progress as ⟨ n2 ⟩
+    scalar_tac
+termination_by n.toNat
+decreasing_by simp_wf; scalar_tac
 
 mutual
 
@@ -22,17 +94,16 @@ end
 
 mutual
 
--- TODO: progress automatically decomposes the post-condition
 theorem even_spec (n : U32) :
   ∃ b, even n = ok b ∧ (b ↔ Even n.val) := by
   rw [even]
   split
   . simp [*]
-  . progress as ⟨ n' .. ⟩
-    progress as ⟨ b .. ⟩
+  . progress as ⟨ n' ⟩
+    progress as ⟨ b ⟩
     simp [*]
     simp [Int.even_sub]
-termination_by n.val.toNat
+termination_by n.toNat
 decreasing_by simp_wf; scalar_tac
 
 theorem odd_spec (n : U32) :
@@ -40,14 +111,117 @@ theorem odd_spec (n : U32) :
   rw [odd]
   split
   . simp [*]
-  . progress as ⟨ n' .. ⟩
-    progress as ⟨ b .. ⟩
+  . progress as ⟨ n' ⟩
+    progress as ⟨ b ⟩
     simp [*]
     simp [Int.even_sub]
-termination_by n.val.toNat
+termination_by n.toNat
 decreasing_by simp_wf; scalar_tac
 
 end
 
+/- [demo::CList]
+   Source: 'tests/src/demo.rs', lines 36:0-36:17 -/
+inductive CList (T : Type) :=
+| CCons : T → CList T → CList T
+| CNil : CList T
+
+/- [demo::list_nth]:
+   Source: 'tests/src/demo.rs', lines 41:0-41:56 -/
+divergent def list_nth (T : Type) (l : CList T) (i : U32) : Result T :=
+  match l with
+  | CList.CCons x tl =>
+    if i = 0#u32
+    then Result.ok x
+    else do
+         let i1 ← i - 1#u32
+         list_nth T tl i1
+  | CList.CNil => Result.fail .panic
+
+-- TODO: list_nth1 (with a loop)
+
+/- [demo::list_tail]:
+   Source: 'tests/src/demo.rs', lines 90:0-90:64 -/
+divergent def list_tail
+  (T : Type) (l : CList T) :
+  Result ((CList T) × (CList T → Result (CList T)))
+  :=
+  match l with
+  | CList.CCons t tl =>
+    do
+    let (c, list_tail_back) ← list_tail T tl
+    let back :=
+      fun ret =>
+        do
+        let tl1 ← list_tail_back ret
+        Result.ok (CList.CCons t tl1)
+    Result.ok (c, back)
+  | CList.CNil => Result.ok (CList.CNil, Result.ok)
+
+open CList
+
+@[simp] def CList.to_list {α : Type} (x : CList α) : List α :=
+  match x with
+  | CNil => []
+  | CCons hd tl => hd :: tl.to_list
+
+theorem list_nth_spec {T : Type} [Inhabited T] (l : CList T) (i : U32)
+  (h : ↑i < l.to_list.len) :
+  ∃ x, list_nth T l i = ok x ∧
+  x = l.to_list.index ↑i
+  := by
+  rw [list_nth]
+  match l with
+  | CNil =>
+    simp_all; scalar_tac
+  | CCons hd tl =>
+    simp_all
+    if hi: i = 0#u32 then
+      simp_all
+    else
+      simp_all
+      progress as ⟨ i1 ⟩
+      progress as ⟨ x ⟩
+      simp_all
+
+theorem list_tail_spec {T : Type} [Inhabited T] (l : CList T) :
+  ∃ back, list_tail T l = ok (CList.CNil, back) ∧
+  ∀ tl', ∃ l', back tl' = ok l' ∧ l'.to_list = l.to_list ++ tl'.to_list := by
+  rw [list_tail]
+  match l with
+  | CNil =>
+    simp_all
+  | CCons hd tl =>
+    simp_all
+    progress as ⟨ back ⟩
+    simp
+    -- Proving the backward function
+    intro tl'
+    progress
+    simp_all
+
+/- Trait declaration: [demo::Counter]
+   Source: 'tests/src/demo.rs', lines 99:0-99:17 -/
+structure Counter (Self : Type) where
+  incr : Self → Result (Usize × Self)
+
+/- [demo::{demo::Counter for usize}::incr]:
+   Source: 'tests/src/demo.rs', lines 104:4-104:31 -/
+def CounterUsize.incr (self : Usize) : Result (Usize × Usize) :=
+  do
+  let self1 ← self + 1#usize
+  Result.ok (self, self1)
+
+/- Trait implementation: [demo::{demo::Counter for usize}]
+   Source: 'tests/src/demo.rs', lines 103:0-103:22 -/
+def CounterUsize : Counter Usize := {
+  incr := CounterUsize.incr
+}
+
+/- [demo::use_counter]:
+   Source: 'tests/src/demo.rs', lines 111:0-111:59 -/
+def use_counter
+  (T : Type) (CounterInst : Counter T) (cnt : T) : Result (Usize × T) :=
+  CounterInst.incr cnt
 
 end Tutorial
